fix the node module and implementation

templates/lockfree/node_impl.v
@@ -6,14 +6,16 @@ From iris.program_logic Require Export atomic.
 From iris.proofmode Require Import tactics.
 From iris.heap_lang Require Import proofmode par.
 From iris.bi.lib Require Import fractional.
+From flows Require Export flows array_util node_module bool_ra gset_seq.
 Set Default Proof Using "All".
-From iris.bi.lib Require Import fractional.
-From flows Require Import skiplist_v1 bool_ra.
 
-Section node_impl.
+Module IMPL1 : NODE_IMPL.
 
-  Parameter L : nat. (* Maxlevels *)
+  Parameter L : nat.
   Parameter randomNum : val.
+
+  Definition MarkT := gmap nat bool.
+  Definition NextT := gmap nat Node.
   
   Definition createNode_rec : val :=
     rec: "cN" "i" "h" "arr" "succs" :=
@@ -34,6 +36,7 @@ Section node_impl.
       createNode_rec #0%nat "h" "arr" "succs";;
       "n".
 
+  (*
   Definition compareKey : val :=
     λ: "n" "k",
       let: "nk" := Fst (! "n") in
@@ -43,7 +46,11 @@ Section node_impl.
         #1
       else
         #2.
-  
+  *)
+  Definition getKey : val :=
+    λ: "n",
+      Fst (! "n").
+
   Definition getHeight : val :=
     λ: "n",
       Snd (! "n").
@@ -102,25 +109,63 @@ Section node_impl.
         else
           NONEV.
 
-  Context `{!heapGS Σ}.
-  Notation iProp := (iProp Σ).
+  Definition changeNext' : val :=
+    rec: "chN" "n" "m" "m'" "p" :=
+      let: "arr" := ! ("n" +ₗ #1) in
+      let: "li" := ! ("arr" +ₗ #0%nat) in
+      let: "res" := ! "li" in
+      if: (Fst "res") then
+        NONEV
+      else
+        if: (Snd "res") = "m" then
+          let: "new" := ref (#false, "m'") in
+          let: "res" := Resolve (CmpXchg ("arr" +ₗ #0%nat) "li" "new") "p" #() in
+          if: Snd "res" then
+            (InjRV #())
+          else
+            "chN" "n" "m" "m'" "p"
+        else
+          NONEV.
 
-  Definition node (n: Node) (h: nat) (mark: gmap nat bool) (next: gmap nat Node) 
-    (k: nat) : iProp :=
+  (* Context `{!heapGS Σ}. *)
+  (* Notation iProp := (iProp Σ). *)
+
+  Definition node Σ (Hg1 : heapGS Σ) (n: Node) (h: nat) (mark: MarkT) (next: NextT) 
+    (k: nat) : iProp Σ :=
     ∃ (arr: loc) (ls: list loc),
        n ↦□ (#k, #h)
     ∗ (n +ₗ 1) ↦□ #arr
     ∗ arr ↦∗ ((fun l => # (LitLoc l)) <$> ls)
-    ∗ ⌜length ls = h⌝
+    ∗ ⌜length ls = h ∧ 0 < h⌝
     ∗ ∀ (l: loc) (i: nat), ⌜ls !! i = Some l⌝ -∗
         l ↦□ (#((mark !!! i): bool), #((next !!! i: loc))).
+  
+  Global Instance node_timeless_proof : ∀ Σ Hg1 n h mark next k, 
+        Timeless (node Σ Hg1 n h mark next k).
+  Proof. try apply _. Qed.
 
+  Lemma node_sep_star Σ Hg1 n h mark next k h' mark' next' k' :
+    node Σ Hg1 n h mark next k -∗ node Σ Hg1 n h' mark' next' k' -∗ False.
+  Proof.
+    iIntros "Hn0 Hn1". 
+    iDestruct "Hn0" as (arr0 ls0) "(#Hk0 & #Hn0 & Harr0 & %Len_vs0 & #Hls0)".
+    iDestruct "Hn1" as (arr1 ls1) "(#Hk1 & #Hn1 & Harr1 & %Len_vs1 & #Hls1)".
+    iDestruct (mapsto_agree with "Hn0 Hn1") as "%H'". inversion H'. clear H'.
+    iDestruct (mapsto_agree with "Hk0 Hk1") as "%H'". inversion H'. clear H'.
+    assert (∃ l0 ls0', ls0 = l0 :: ls0') as [l0 [ls0' Def_ls0]].
+    { destruct ls0. rewrite /= in Len_vs0. lia. by exists l, ls0. }
+    rewrite Def_ls0 array_cons. iDestruct "Harr0" as "(Harr0 & Harr0')". 
+    assert (∃ l1 ls1', ls1 = l1 :: ls1') as [l1 [ls1' Def_ls1]].
+    { destruct ls1. rewrite /= in Len_vs1. lia. by exists l, ls1. }
+    rewrite Def_ls1 array_cons. iDestruct "Harr1" as "(Harr1 & Harr1')".
+    iCombine "Harr0 Harr1" as "H'". iPoseProof (mapsto_valid with "H'") as "%".
+    exfalso; try done.
+  Qed.
+
+  (*
   Definition is_array (array : loc) (xs : list Node) : iProp :=
     let vs := (fun n => # (LitLoc n)) <$> xs
     in array ↦∗ vs.
-
-  Parameter randomNum_spec : ∀ (n: nat),
-  ⊢  {{{ True }}} randomNum #n {{{ (n': nat), RET #n'; ⌜0 < n' < n⌝ }}}.
 
   Lemma array_store E (i : nat) (v : Node) arr (xs : list Node) :
     {{{ ⌜i < length xs⌝ ∗ ▷ is_array arr xs }}}
@@ -142,9 +187,13 @@ Section node_impl.
     rewrite -> fmap_replicate.
     (* iAssumption. *)
   Admitted.
+  *)
 
-  Lemma createNode_rec_spec (arr succs: loc) (ls ss: list Node) (h i: nat) :
-  ⊢  {{{ is_array succs ss 
+  Parameter randomNum_spec : ∀ Σ (Hg1: heapGS Σ) (n: nat),
+  ⊢  {{{ True }}} randomNum #n {{{ (n': nat), RET #n'; ⌜0 < n' < n⌝ }}}.
+
+  Lemma createNode_rec_spec Σ (Hg1 : heapGS Σ) (arr succs: loc) (ls ss: list Node) (h i: nat) :
+  ⊢  {{{ is_array Σ Hg1 succs ss 
          ∗ arr ↦∗ ((fun l => # (LitLoc l)) <$> ls)
          ∗ ⌜length ls = h⌝
          ∗ ⌜h <= length ss⌝
@@ -154,7 +203,7 @@ Section node_impl.
            createNode_rec #i #h #arr #succs
       {{{ (ls': list Node),
           RET #();
-              is_array succs ss
+              is_array Σ Hg1 succs ss
             ∗ arr ↦∗ ((fun l => # (LitLoc l)) <$> ls')
             ∗ ⌜length ls' = h⌝
             ∗ ∀ (l: loc) (j: nat), 
@@ -201,13 +250,15 @@ Section node_impl.
       iPureIntro; lia.
   Qed.
 
-  Lemma createNode_spec (succs: loc) ss (k: nat) :
-  ⊢  {{{ is_array succs ss ∗ ⌜length ss = L⌝ }}}
+  Lemma createNode_spec Σ (Hg1 : heapGS Σ) (succs: loc) ss (k: nat) :
+  ⊢  {{{ is_array Σ Hg1 succs ss ∗ ⌜length ss = L⌝ }}}
            createNode #k #succs
         {{{ (n: Node) (h: nat) mark next,
             RET #n;
-              is_array succs ss
-            ∗ node n h mark next k  
+              is_array Σ Hg1 succs ss
+            ∗ node Σ Hg1 n h mark next k
+            ∗ ⌜0 < h < L⌝
+            ∗ ⌜dom mark = gset_seq 0 (h-1)⌝ ∗ ⌜dom next = gset_seq 0 (h-1)⌝
             ∗ (⌜∀ i, i < h → mark !! i = Some false⌝)
             ∗ (⌜∀ i, i < h → next !! i = Some (ss !!! i)⌝) }}}.
   Proof.
@@ -224,7 +275,7 @@ Section node_impl.
     iApply (wp_store_offset _ _ n 1 with "Hn").
     { apply lookup_lt_is_Some_2. rewrite replicate_length. lia. }
     iIntros "!> Hn". wp_pures.
-    wp_apply (createNode_rec_spec _ _ _ _ h _ with "[Hsuccs Harr]").
+    wp_apply (createNode_rec_spec _ _ _ _ _ _ h _ with "[Hsuccs Harr]").
     { assert (replicate h #n = (λ l : loc, #l) <$> (replicate h n)) as ->.
       { apply list_eq. intros i'. rewrite list_lookup_fmap. 
         destruct (decide (i' < h)) as [Hi | Hi].
@@ -239,8 +290,9 @@ Section node_impl.
       iSplitR. iPureIntro; lia.
       iIntros (l j)"%Hlj %Hj". exfalso; lia. }
     iIntros (ls) "(Hsuccs & Harr & %Length_ls & Hls)".
-    assert (∃ (m: gmap nat bool), ∀ i, i < h → m !! i = Some false) as 
-      [mark Def_mark].
+    assert (∃ (m: gmap nat bool), (∀ i, i < h → m !! i = Some false) 
+      ∧ dom m = gset_seq 0 (h-1)) as 
+      [mark [Def_mark Dom_mark]].
     { Fixpoint f n (res: gmap nat bool) := 
         match n with S n' => f n' (<[n' := false]> res) | 0 => res end.
       set m := f h ∅.
@@ -257,9 +309,17 @@ Section node_impl.
             assert (i < n) as H'%H'' by lia. by rewrite H'.
           + assert (¬ i < n) as H'%H'' by lia. rewrite H'.
             rewrite lookup_insert_ne; try (done || lia). }
-      exists m. apply  H'. }
-    assert (∃ (nx: gmap nat Node), ∀ i, i < h → nx !! i = Some (ss !!! i)) as 
-      [next Def_next].
+      exists m. split. apply H'. pose proof H' h ∅ as H'. 
+      rewrite -/m in H'. apply set_eq_subseteq. split.
+      intros j Hj. destruct (decide (j < h)) as [Hj' | Hj']. 
+      rewrite elem_of_gset_seq. lia. apply H' in Hj'. 
+      rewrite lookup_empty -not_elem_of_dom in Hj'. done.
+      intros j Hj. rewrite elem_of_gset_seq in Hj. 
+      assert (j < h) as H'' by lia. apply H' in H''.
+      rewrite elem_of_dom H''. done. }
+    assert (∃ (nx: gmap nat Node), (∀ i, i < h → nx !! i = Some (ss !!! i))
+      ∧ dom nx = gset_seq 0 (h-1)) as 
+      [next [Def_next Dom_next]].
     { Fixpoint f' (l: list Node) n (res: gmap nat Node) := 
         match n with S n' => f' l n' (<[n':= l !!! n']> res) | 0 => res end.
       set nx := f' ss h ∅.
@@ -276,10 +336,17 @@ Section node_impl.
             assert (i < n) as H'%H'' by lia. by rewrite H'.
           + assert (¬ i < n) as H'%H'' by lia. rewrite H'.
             rewrite lookup_insert_ne; try (done || lia). }
-      exists nx. apply H'. }
+      exists nx. split. apply H'. pose proof H' h ∅ as H'. 
+      rewrite -/nx in H'. apply set_eq_subseteq. split.
+      intros j Hj. destruct (decide (j < h)) as [Hj' | Hj']. 
+      rewrite elem_of_gset_seq. lia. apply H' in Hj'. 
+      rewrite lookup_empty -not_elem_of_dom in Hj'. done.
+      intros j Hj. rewrite elem_of_gset_seq in Hj. 
+      assert (j < h) as H'' by lia. apply H' in H''.
+      rewrite elem_of_dom H''. done. }
     wp_pures. iApply ("Hpost" $! n h mark next).
     iFrame "Hsuccs". iSplitL; last first.
-    { iPureIntro; try done. }  
+    { iPureIntro. repeat split; try (done || lia). }  
     iExists arr, ls.
     assert (<[1:=#arr]> (replicate 2 (#k, #h)%V) = (#k, #h)%V :: #arr :: []) as ->.
     { rewrite /replicate /=. done. }
@@ -290,7 +357,7 @@ Section node_impl.
         lia. destruct n; try done. } iFrame. }
     iDestruct (mapsto_persist with "Hk") as ">Hk".
     iDestruct (mapsto_persist with "Hn") as ">Hn".
-    iFrame "Hn Hk Harr". iSplitR. by iPureIntro.
+    iFrame "Hn Hk Harr". iSplitR. iPureIntro. split; try (done || lia).
     iModIntro. iIntros (l j)"%Hlj".
     assert (j < h) as j_lt_h. { by rewrite -Length_ls -lookup_lt_is_Some Hlj /=. }
     rewrite lookup_total_alt Def_mark /=; try done.
@@ -298,6 +365,7 @@ Section node_impl.
     iDestruct ("Hls" with "[%] [%]") as "H'"; try done.
   Qed.
 
+  (*
   Lemma compareKey_spec (n: Node) (k': nat) :
     ⊢ <<{ ∀∀ h mark next k, node n h mark next k }>>
            compareKey #n #k' @ ∅
@@ -350,11 +418,12 @@ Section node_impl.
           #(LitInt (Z.of_nat k')))) eqn: H''; wp_pures; try done.
         rewrite bool_decide_eq_true in H''. inversion H''. lia.
   Qed.
+  *)
 
-  Lemma getHeight_spec (n: Node) (i: nat) :
-    ⊢ <<{ ∀∀ h mark next k, node n h mark next k }>>
+  Lemma getHeight_spec Σ Hg1 (n: Node) :
+    ⊢ <<{ ∀∀ h mark next k, node Σ Hg1 n h mark next k }>>
           getHeight #n @ ∅
-      <<{ node n h mark next k | RET #h }>>.
+      <<{ node Σ Hg1 n h mark next k | RET #h }>>.
   Proof.
     iIntros (Φ) "AU".
     wp_lam. wp_pures. wp_bind (! _)%E.
@@ -366,11 +435,26 @@ Section node_impl.
     iModIntro. wp_pures. done.
   Qed.
 
-  Lemma findNext_spec (n: Node) (i: nat) :
-    ⊢ <<{ ∀∀ h mark next k, node n h mark next k ∗ ⌜i < h⌝ }>>
-          findNext #n #i @⊤
+  Lemma getKey_spec Σ Hg1 (n: Node) :
+    ⊢ <<{ ∀∀ h mark next k, node Σ Hg1 n h mark next k }>>
+          getKey #n @ ∅
+      <<{ node Σ Hg1 n h mark next k | RET #k }>>.
+  Proof.
+    iIntros (Φ) "AU".
+    wp_lam. wp_pures. wp_bind (! _)%E.
+    iMod "AU" as (h0 m0 nx0 k0) "[Node [_ Hclose]]".
+    iDestruct "Node" as (arr0 ls0) "(#Hk0 & #Hn0 & Harr & %Len_vs0 & #Hls0)".
+    wp_load. 
+    iMod ("Hclose" with "[Harr]") as "AU".
+    { iFrame "%". iExists arr0, ls0. iFrame "∗#%". }
+    iModIntro. wp_pures. done.
+  Qed.
+
+  Lemma findNext_spec Σ Hg1 (n: Node) (i: nat) :
+    ⊢ <<{ ∀∀ h mark next k, node Σ Hg1 n h mark next k ∗ ⌜i < h⌝ }>>
+          findNext #n #i @ ∅
       <<{ ∃∃ (m: bool) (n': Node),
-              node n h mark next k ∗ ⌜mark !!! i = m⌝ ∗ ⌜next !!! i = n'⌝ |
+              node Σ Hg1 n h mark next k ∗ ⌜mark !!! i = m⌝ ∗ ⌜next !!! i = n'⌝ |
               RET (#m, #n') }>>.
   Proof.
     iIntros (Φ) "AU".
@@ -386,7 +470,7 @@ Section node_impl.
     iDestruct (mapsto_agree with "[$Hn0] [$Hn1]") as "%H'". 
     inversion H'; subst arr1; clear H'.
     assert (∃ li, ls1 !! i = Some li) as [li Def_li].
-    { apply lookup_lt_is_Some. by rewrite Len_vs1. }  
+    { apply lookup_lt_is_Some. destruct Len_vs1 as [-> _]. done.  }  
     wp_apply (wp_load_offset _ _ _ (DfracOwn (pos_to_Qp 1)) _ 
         _ #li with "[Harr]"); try done.
     { by rewrite list_lookup_fmap Def_li /=. }
@@ -398,11 +482,11 @@ Section node_impl.
     iModIntro. wp_pures. wp_load. by wp_pures.
   Qed.
   
-  Lemma markNode_spec (n: Node) (i: nat) :
-    ⊢  <<{ ∀∀ h mark next k, node n h mark next k ∗ ⌜i < h⌝ }>>
-            markNode #n #i @⊤
+  Lemma markNode_spec Σ Hg1 (n: Node) (i: nat) :
+    ⊢  <<{ ∀∀ h mark next k, node Σ Hg1 n h mark next k ∗ ⌜i < h⌝ }>>
+            markNode #n #i @ ∅
       <<{ ∃∃ (success: bool) mark',
-              node n h mark' next k
+              node Σ Hg1 n h mark' next k
             ∗ (match success with true => ⌜mark !!! i = false
                                             ∧ mark' = <[i := true]> mark⌝
                                 | false => ⌜mark !!! i = true
@@ -423,7 +507,7 @@ Section node_impl.
     iDestruct (mapsto_agree with "[$Hn0] [$Hn1]") as "%H'". 
     inversion H'; subst arr1; clear H'.
     assert (∃ li, ls1 !! i = Some li) as [li Def_li].
-    { apply lookup_lt_is_Some. by rewrite Len_vs1. }  
+    { apply lookup_lt_is_Some. by destruct Len_vs1 as [-> _]. }  
     wp_apply (wp_load_offset _ _ _ (DfracOwn (pos_to_Qp 1)) _ 
         _ #li with "[Harr]"); try done.
     { by rewrite list_lookup_fmap Def_li /=. }
@@ -450,7 +534,7 @@ Section node_impl.
       iDestruct (mapsto_agree with "[$Hn0] [$Hn2]") as "%H'". 
       inversion H'; subst arr2; clear H'.
       assert (∃ li', ls2 !! i = Some li') as [li' Def_li'].
-      { apply lookup_lt_is_Some. by rewrite Len_vs2.  }
+      { apply lookup_lt_is_Some. by destruct Len_vs2 as [-> _].  }
       destruct (decide (li' = li)) as [-> | Des_li].
       + wp_apply (wp_cmpxchg_suc_offset _ _ _ _ _ _ with "[Harr]"); 
           try done.
@@ -467,7 +551,8 @@ Section node_impl.
           iSplitL "Harr". 
           assert (((λ l : loc, #l) <$> <[i:=li_new]> ls2) = 
             <[i:=#li_new]> ((λ l : loc, #l) <$> ls2)) as ->.
-          { apply list_eq. intros i'. destruct (decide (i' = i)) as [-> | Hi'].
+          { destruct Len_vs2 as [Len_vs2 _]. apply list_eq. intros i'. 
+            destruct (decide (i' = i)) as [-> | Hi'].
             rewrite list_lookup_fmap !list_lookup_insert /=. done.
             by rewrite fmap_length Len_vs2. by rewrite Len_vs2. 
             rewrite list_lookup_fmap !list_lookup_insert_ne /=; try done.
@@ -477,7 +562,7 @@ Section node_impl.
           assert (<[i:=true]> m2 !!! i = true) as ->.
           by rewrite lookup_total_insert.
           rewrite list_lookup_insert in Hlj. inversion Hlj.
-          rewrite H1; try done. by rewrite Len_vs2.
+          rewrite H1; try done. by destruct Len_vs2 as [-> _].
           assert (<[i:=true]> m2 !!! j = m2 !!! j) as ->.
           by rewrite lookup_total_insert_ne.
           rewrite list_lookup_insert_ne in Hlj; try done.
@@ -497,12 +582,12 @@ Section node_impl.
         iModIntro. wp_pures. by iApply "IH".
   Qed.  
 
-  Lemma markNode_proph_spec (n: Node) (p: proph_id) pvs :
+  Lemma markNode_proph_spec Σ Hg1 (n: Node) (p: proph_id) pvs :
     ⊢ proph p pvs -∗ 
-      <<{ ∀∀ h mark next k, node n h mark next k ∗ ⌜0 < h⌝ }>>
+      <<{ ∀∀ h mark next k, node Σ Hg1 n h mark next k ∗ ⌜0 < h⌝ }>>
             markNode' #n #p @ ∅
       <<{ ∃∃ (success: bool) mark' prf pvs',
-              node n h mark' next k
+              node Σ Hg1 n h mark' next k
             ∗ proph p pvs'
             ∗ ⌜Forall (λ x, ∃ v1, x = ((v1, #false)%V, #())) prf⌝
             ∗ (match success with 
@@ -528,7 +613,7 @@ Section node_impl.
     iDestruct (mapsto_agree with "[$Hn0] [$Hn1]") as "%H'". 
     inversion H'; subst arr1; clear H'.
     assert (∃ li, ls1 !! 0 = Some li) as [li Def_li].
-    { apply lookup_lt_is_Some. by rewrite Len_vs1. }  
+    { apply lookup_lt_is_Some. by destruct Len_vs1 as [-> _]. }  
     wp_apply (wp_load_offset _ _ _ (DfracOwn (pos_to_Qp 1)) _ 
         _ #li with "[Harr]"); try done.
     { by rewrite list_lookup_fmap Def_li /=. }
@@ -582,7 +667,8 @@ Section node_impl.
           assert (<[0:=true]> m2 !!! 0 = true) as ->.
           by rewrite lookup_total_insert.
           rewrite list_lookup_insert in Hlj. inversion Hlj.
-          rewrite H1; try done. by rewrite Def_ls2 Len_vs2.
+          rewrite H1; try done. destruct Len_vs2 as [Len_vs2 _]. 
+          by rewrite Def_ls2 Len_vs2.
           assert (<[0:=true]> m2 !!! j = m2 !!! j) as ->.
           by rewrite lookup_total_insert_ne.
           rewrite list_lookup_insert_ne in Hlj; try done.
@@ -617,11 +703,11 @@ Section node_impl.
           done.
   Qed.
 
-  Lemma changeNext_spec (n m m': Node) (i: nat) :
-    ⊢  <<{ ∀∀ h mark next k, node n h mark next k ∗ ⌜i < h⌝ }>>
-            changeNext #n #m #m' #i @⊤
+  Lemma changeNext_spec Σ Hg1 (n m m': Node) (i: nat) :
+    ⊢  <<{ ∀∀ h mark next k, node Σ Hg1 n h mark next k ∗ ⌜i < h⌝ }>>
+            changeNext #n #m #m' #i @ ∅
       <<{ ∃∃ (success: bool) next',
-              node n h mark next' k
+              node Σ Hg1 n h mark next' k
             ∗ (match success with true => ⌜next !!! i = m 
                                             ∧ mark !!! i = false
                                             ∧ next' = <[i := m']> next⌝
@@ -644,7 +730,7 @@ Section node_impl.
     iDestruct (mapsto_agree with "[$Hn0] [$Hn1]") as "%H'". 
     inversion H'; subst arr1; clear H'.
     assert (∃ li, ls1 !! i = Some li) as [li Def_li].
-    { apply lookup_lt_is_Some. by rewrite Len_vs1. }  
+    { apply lookup_lt_is_Some. by destruct Len_vs1 as [-> _]. }  
     wp_apply (wp_load_offset _ _ _ (DfracOwn (pos_to_Qp 1)) _ 
         _ #li with "[Harr]"); try done.
     { by rewrite list_lookup_fmap Def_li /=. }
@@ -680,7 +766,7 @@ Section node_impl.
         iDestruct (mapsto_agree with "[$Hn0] [$Hn2]") as "%H'". 
         inversion H'; subst arr2; clear H'.
         assert (∃ li', ls2 !! i = Some li') as [li' Def_li'].
-        { apply lookup_lt_is_Some. by rewrite Len_vs2. }
+        { apply lookup_lt_is_Some. by destruct Len_vs2 as [-> _]. }
         destruct (decide (li' = li)) as [-> | Des_li].
         * wp_apply (wp_cmpxchg_suc_offset _ _ _ _ _ _ with "[Harr]"); 
             try done.
@@ -696,7 +782,7 @@ Section node_impl.
             iSplitL. 
             assert (((λ l : loc, #l) <$> <[i:=li_new]> ls2) = 
                       <[i:=#li_new]> ((λ l : loc, #l) <$> ls2)) as ->.
-            { apply list_eq. intros i'. 
+            { destruct Len_vs2 as [Len_vs2 _]. apply list_eq. intros i'. 
               destruct (decide (i' = i)) as [-> | Hi'].
               rewrite list_lookup_fmap !list_lookup_insert /=. done.
               by rewrite fmap_length Len_vs2. by rewrite Len_vs2. 
@@ -728,4 +814,136 @@ Section node_impl.
           iModIntro. wp_pures. by iApply "IH".
   Qed.
 
-End node_impl.
+  Lemma changeNext_proph_spec Σ (Hg1 : heapGS Σ) (n m m': Node) (p: proph_id) pvs :
+  ⊢ proph p pvs -∗
+    <<{ ∀∀ h mark next k, node Σ Hg1 n h mark next k ∗ ⌜0 < h⌝ }>>
+          changeNext' #n #m #m' #p @ ∅
+    <<{ ∃∃ (success: bool) next' prf pvs',
+            node Σ Hg1 n h mark next' k
+          ∗ proph p pvs'
+          ∗ ⌜Forall (λ x, ∃ v1, x = ((v1, #false)%V, #())) prf⌝
+          ∗ (match success with 
+              true => ⌜next !!! 0 = m 
+                      ∧ mark !!! 0 = false
+                      ∧ next' = <[0 := m']> next
+                      ∧ (∃ v1, pvs = prf ++ [((v1, #true)%V, #())] ++ pvs')⌝
+            | false => ⌜(next !!! 0 ≠ m ∨ mark !!! 0 = true)
+                        ∧ next' = next
+                        ∧ pvs = prf ++ pvs'⌝ end) |
+            RET (match success with true => SOMEV #() 
+                                  | false => NONEV end) }>>.
+  Proof.
+    iIntros "Hproph" (Φ) "AU". iLöb as "IH" forall (pvs).
+    wp_lam. wp_pures. wp_bind (! _)%E.
+    iMod "AU" as (h0 m0 nx0 k0) "[(Node&%Hi0) [Hclose _]]".
+    iDestruct "Node" as (arr0 ls0) "(#Hk0 & #Hn0 & Harr & %Len_vs0 & #Hls0)".
+    wp_load. 
+    iMod ("Hclose" with "[Harr]") as "AU".
+    { iSplitL; last by iPureIntro. iExists arr0, ls0. iFrame "∗#%". }
+    iModIntro. wp_pures. wp_bind (! _)%E.
+    iMod "AU" as (h1 m1 nx1 k1) "[(Node&%Hi1) HAU]".
+    iDestruct "Node" as (arr1 ls1) "(#Hk1 & #Hn1 & Harr & %Len_vs1 & #Hls1)".
+    iDestruct (mapsto_agree with "[$Hn0] [$Hn1]") as "%H'". 
+    inversion H'; subst arr1; clear H'.
+    assert (∃ li, ls1 !! 0 = Some li) as [li Def_li].
+    { apply lookup_lt_is_Some. by destruct Len_vs1 as [-> _]. }  
+    wp_apply (wp_load_offset _ _ _ (DfracOwn (pos_to_Qp 1)) _ 
+        _ #li with "[Harr]"); try done.
+    { by rewrite list_lookup_fmap Def_li /=. }
+    iIntros "Harr".
+    iDestruct ("Hls1" with "[%]") as "H'". apply Def_li.
+    destruct (decide (m1 !!! 0 = true)) as [Hmi | Hmi].
+    - iDestruct "HAU" as "[_ Hclose]".
+      iSpecialize ("Hclose" $! false nx1).
+      iMod ("Hclose" with "[Harr Hproph]") as "HΦ".
+      { iFrame. iSplitL. iExists arr0, ls1. iFrame "∗#%".
+        iPureIntro; split; try done. repeat split; try done. by right. }
+      iModIntro. wp_pures. wp_load. wp_pures.
+      rewrite Hmi. wp_pures. done.
+    - apply not_true_is_false in Hmi. rewrite Hmi.
+      destruct (decide (nx1 !!! 0 = m)) as [Hnx1_i | Hnx1_i]; last first.
+      + iDestruct "HAU" as "[_ Hclose]".
+        iSpecialize ("Hclose" $! false nx1).
+        iMod ("Hclose" with "[Harr Hproph]") as "AU".
+        { iFrame. iSplitL. iExists arr0, ls1. iFrame "∗#%". iPureIntro.
+          repeat split; try done. by left. }
+        iModIntro. wp_pures. wp_load. wp_pures.
+        rewrite bool_decide_eq_false_2; last first. { by intros [=]. }
+        wp_pures. done.
+      + iDestruct "HAU" as "[Hclose _]".
+        iMod ("Hclose" with "[Harr]") as "AU".
+        { iSplitL; last by iPureIntro. iExists arr0, ls1. iFrame "∗#%". }
+        iModIntro. wp_pures. wp_load. wp_pures.
+        rewrite bool_decide_eq_true_2; last first. { by rewrite Hnx1_i. }
+        wp_pures. wp_alloc li_new as "Hnew". wp_pures.
+        wp_bind (Resolve _ _ _)%E. 
+        iMod "AU" as (h2 m2 nx2 k2) "[(Node&%Hi2) HAU]".
+        iDestruct "Node" as (arr2 ls2) "(#Hk2 & #Hn2 & Harr & %Len_vs2 & #Hls2)".
+        iDestruct (mapsto_agree with "[$Hn0] [$Hn2]") as "%H'". 
+        inversion H'; subst arr2; clear H'.
+        destruct ls2 as [|li' ls2'] eqn: Def_ls2. 
+        { rewrite /= in Len_vs2. exfalso; lia. }
+        assert (ls2 !! 0 = Some li') as Def_li'.
+        { by rewrite Def_ls2 /=. }
+        assert (((λ l : loc, #l) <$> li' :: ls2') = 
+          #li' :: ((λ l : loc, #l) <$> ls2')) as ->.
+        { by rewrite fmap_cons. } rewrite array_cons. 
+        iDestruct "Harr" as "(Harr0 & Harr)".
+        assert (arr0 +ₗ 0%nat = arr0) as ->. { by rewrite Loc.add_0. }
+        destruct (decide (li' = li)) as [-> | Des_li].
+        * wp_apply (wp_resolve_cmpxchg_suc with "[$Harr0 $Hproph]").
+          { by left. }
+          iIntros "H''". iDestruct "H''" as (pvs')"(%Hpvs' & Hproph & Harr0)".
+          iDestruct "HAU" as "[_ Hclose]".
+          iSpecialize ("Hclose" $! true (<[0:=m']> nx2)).
+          iDestruct (mapsto_persist with "Hnew") as ">#Hnew'".
+          iDestruct ("Hls2" with "[%]") as "H''". rewrite -Def_ls2. apply Def_li'.
+          iDestruct (mapsto_agree with "H' H''") as "%H'". inversion H'.
+          iMod ("Hclose" with "[Harr Harr0 Hproph]") as "HΦ".
+          { iFrame "Hproph". iSplitL. iExists arr0, (<[0:= li_new]> ls2). iFrame "#".
+            iSplitL. assert (((λ l : loc, #l) <$> <[0:=li_new]> ls2) = 
+              #li_new :: ((λ l : loc, #l) <$> ls2')) as ->.
+            { rewrite Def_ls2 /=. apply f_equal. done. } 
+            rewrite array_cons. iFrame. 
+            iSplitR. { iPureIntro. by rewrite insert_length Def_ls2. }
+            iIntros (l j)"%Hlj". destruct (decide (j = 0)) as [-> | Hj].
+            rewrite list_lookup_insert in Hlj. inversion Hlj. subst l.
+            assert (m2 !!! 0%nat = false) as -> by done.
+            assert ((<[0%nat:=m']> nx2 !!! 0%nat : loc) = m') as ->.
+            by rewrite lookup_total_insert.
+            rewrite H1; try done. destruct Len_vs2 as [Len_vs2 _]. 
+            by rewrite Def_ls2 Len_vs2.
+            assert ((<[0%nat:=m']> nx2 !!! j : loc) = nx2 !!! j) as ->.
+            by rewrite lookup_total_insert_ne.
+            rewrite list_lookup_insert_ne in Hlj; try done.
+            iClear "H' H''".
+            iDestruct ("Hls2" with "[%]") as "H'". rewrite -Def_ls2. apply Hlj.
+            iFrame "#". iPureIntro. repeat split; try done. by rewrite -H1.
+            exists #li. rewrite Hpvs'. clear; set_solver. }
+          iModIntro. wp_pures. done.
+        * wp_apply (wp_resolve_cmpxchg_fail with "[$Harr0 $Hproph]").
+          { by intros [=->]. }
+          { by left. }
+          iIntros "H''". iDestruct "H''" as (pvs')"(%Hpvs' & Hproph & Harr0)".
+          iDestruct "HAU" as "[Hclose _]".
+          iMod ("Hclose" with "[Harr Harr0]") as "AU".
+          { iSplitL; last by iPureIntro. iExists arr0, (li' :: ls2'). iFrame "∗#%". }
+          iModIntro. wp_pures. iApply ("IH" with "[$Hproph] [AU]"); try done.
+          iAuIntro. rewrite /atomic_acc /=. iClear "#". 
+          iMod "AU" as (h3 m3 nx3 k3)"[H' H'']". iModIntro.
+          iExists h3, m3, nx3, k3. iFrame "H'". iSplit.
+          ** iDestruct "H''" as "[H'' _]". iApply "H''".
+          ** iDestruct "H''" as "[_ H'']". iIntros (res nx3' prf pvs'').
+            iIntros "(Node & Hproph & %Hprf & Hres)". 
+            iSpecialize ("H''" $! res nx3' (((#li', #false)%V, #()) :: prf) pvs'').
+            iMod ("H''" with "[Node Hproph Hres]") as "HΦ"; try done.
+            iFrame "Node Hproph". iSplitR. iPureIntro. 
+            rewrite Forall_cons; split; try done. by exists #li'.
+            destruct res; iDestruct "Hres" as "%H'"; iPureIntro; 
+              repeat split; try apply H'. destruct H' as (_&_&_&[v1 Def_pvs']).
+            rewrite Def_pvs' in Hpvs'. exists v1. rewrite Hpvs'. done.
+            destruct H' as (_&_&Def_pvs'). rewrite Def_pvs' in Hpvs'.
+            rewrite Hpvs'. clear; set_solver.
+  Qed.
+
+End IMPL1.
