templates/lockfree/node_module.v
@@ -12,50 +12,54 @@ From flows Require Import array_util bool_ra gset_seq.
 
 Module Type NODE_IMPL.
 
+  Parameter L : nat.
+
   Definition MarkT := gmap nat bool.
   Definition NextT := gmap nat Node.
 
-  Parameter node : ∀ Σ, Node → nat → MarkT → NextT → nat → iProp Σ.
-  #[global] Declare Instance node_timeless_proof : ∀ Σ n h mark next k, 
-    Timeless (node Σ n h mark next k).
+  Parameter node : ∀ Σ, heapGS Σ → Node → nat → MarkT → NextT → nat → iProp Σ.
+  #[global] Declare Instance node_timeless_proof : ∀ Σ Hg1 n h mark next k, 
+    Timeless (node Σ Hg1 n h mark next k).
 
-  Parameter node_sep_star: ∀ Σ n h mark next k h' mark' next' k',
-    node Σ n h mark next k -∗ node Σ n h' mark' next' k' -∗ False.
+  Parameter node_sep_star: ∀ Σ Hg1 n h mark next k h' mark' next' k',
+    node Σ Hg1 n h mark next k -∗ node Σ Hg1 n h' mark' next' k' -∗ False.
 
-  Parameter inContents : val.
+  (* Parameter inContents : val. *)
   Parameter findNext : val.
   Parameter changeNext : val.
+  Parameter changeNext' : val.
   Parameter markNode : val.
-  Parameter compareKey : val.
+  Parameter markNode' : val.
+  (* Parameter compareKey : val. *)
   Parameter getKey : val.
   Parameter createNode : val.
   Parameter getHeight : val.
-  Parameter permute_levels : val.
+  (* Parameter permute_levels : val. *)
 
-  Parameter createNode_spec : ∀ Σ (H' : heapGS Σ) (succs: loc) ss (L k: nat),
+  Parameter createNode_spec : ∀ Σ Hg1 (succs: loc) ss (k: nat),
   ⊢  {{{ is_array Σ _ succs ss ∗ ⌜length ss = L⌝ }}}
            createNode #k #succs
         {{{ (n: Node) (h: nat) mark next,
             RET #n;
               is_array Σ _ succs ss
-            ∗ node Σ n h mark next k
+            ∗ node Σ Hg1 n h mark next k
             ∗ ⌜0 < h < L⌝
             ∗ ⌜dom mark = gset_seq 0 (h-1)⌝ ∗ ⌜dom next = gset_seq 0 (h-1)⌝
             ∗ (⌜∀ i, i < h → mark !! i = Some false⌝)
             ∗ (⌜∀ i, i < h → next !! i = Some (ss !!! i)⌝) }}}.
 
-  Parameter findNext_spec : ∀ Σ (H' : heapGS Σ) (n: Node) (i: nat),
-    ⊢ <<{ ∀∀ h mark next k, node Σ n h mark next k ∗ ⌜i < h⌝ }>>
+  Parameter findNext_spec : ∀ Σ Hg1 (n: Node) (i: nat),
+    ⊢ <<{ ∀∀ h mark next k, node Σ Hg1 n h mark next k ∗ ⌜i < h⌝ }>>
           findNext #n #i @ ∅
       <<{ ∃∃ (m: bool) (n': Node),
-              node Σ n h mark next k ∗ ⌜mark !!! i = m⌝ ∗ ⌜next !!! i = n'⌝ |
+              node Σ Hg1 n h mark next k ∗ ⌜mark !!! i = m⌝ ∗ ⌜next !!! i = n'⌝ |
               RET (#m, #n') }>>.
 
-  Parameter changeNext_spec : ∀ Σ (H' : heapGS Σ) (n m m': Node) (i: nat),
-    ⊢  <<{ ∀∀ h mark next k, node Σ n h mark next k ∗ ⌜i < h⌝ }>>
+  Parameter changeNext_spec : ∀ Σ Hg1 (n m m': Node) (i: nat),
+    ⊢  <<{ ∀∀ h mark next k, node Σ Hg1 n h mark next k ∗ ⌜i < h⌝ }>>
             changeNext #n #m #m' #i @ ∅
       <<{ ∃∃ (success: bool) next',
-              node Σ n h mark next' k
+              node Σ Hg1 n h mark next' k
             ∗ (match success with true => ⌜next !!! i = m 
                                             ∧ mark !!! i = false
                                             ∧ next' = <[i := m']> next⌝
@@ -65,12 +69,12 @@ Module Type NODE_IMPL.
               RET (match success with true => SOMEV #() 
                                     | false => NONEV end) }>>.
 
-  Parameter changeNext_proph_spec : ∀ Σ (H' : heapGS Σ) (n m m': Node) (p: proph_id) pvs,
+  Parameter changeNext_proph_spec : ∀ Σ Hg1 (n m m': Node) (p: proph_id) pvs,
     ⊢ proph p pvs -∗
-      <<{ ∀∀ h mark next k, node Σ n h mark next k ∗ ⌜0 < h⌝ }>>
-            changeNext #n #m #m' #p @ ∅
+      <<{ ∀∀ h mark next k, node Σ Hg1 n h mark next k ∗ ⌜0 < h⌝ }>>
+            changeNext' #n #m #m' #p @ ∅
       <<{ ∃∃ (success: bool) next' prf pvs',
-              node Σ n h mark next' k
+              node Σ Hg1 n h mark next' k
             ∗ proph p pvs'
             ∗ ⌜Forall (λ x, ∃ v1, x = ((v1, #false)%V, #())) prf⌝
             ∗ (match success with 
@@ -84,26 +88,16 @@ Module Type NODE_IMPL.
               RET (match success with true => SOMEV #() 
                                     | false => NONEV end) }>>.
 
-  Parameter compareKey_spec : ∀ Σ (H' : heapGS Σ) (n: Node) (k': nat),
-    ⊢ <<{ ∀∀ h mark next k, node Σ n h mark next k }>>
-           compareKey #n #k' @ ∅
-     <<{ ∃∃ (res: nat),
-            node Σ n h mark next k 
-          ∗ ⌜if decide (res = 0) then k < k'
-             else if decide (res = 1) then k = k'
-             else k > k'⌝ |
-         RET #res }>>.
-
-  Parameter getKey_spec : ∀ Σ (H' : heapGS Σ) (n: Node),
-    ⊢ <<{ ∀∀ h mark next k, node Σ n h mark next k }>>
+  Parameter getKey_spec : ∀ Σ Hg1 (n: Node),
+    ⊢ <<{ ∀∀ h mark next k, node Σ Hg1 n h mark next k }>>
            getKey #n @ ∅
-     <<{ node Σ n h mark next k | RET #k }>>.
+     <<{ node Σ Hg1 n h mark next k | RET #k }>>.
 
-  Parameter markNode_spec : ∀ Σ (n: Node) (H' : heapGS Σ) (i: nat),
-    ⊢ <<{ ∀∀ h mark next k, node Σ n h mark next k ∗ ⌜i < h⌝ }>>
+  Parameter markNode_spec : ∀ Σ Hg1 (n: Node) (i: nat),
+    ⊢ <<{ ∀∀ h mark next k, node Σ Hg1 n h mark next k ∗ ⌜i < h⌝ }>>
             markNode #n #i @ ∅
       <<{ ∃∃ (success: bool) mark',
-              node Σ n h mark' next k
+              node Σ Hg1 n h mark' next k
             ∗ (match success with true => ⌜mark !!! i = false
                                             ∧ mark' = <[i := true]> mark⌝
                                 | false => ⌜mark !!! i = true
@@ -112,12 +106,12 @@ Module Type NODE_IMPL.
                                     | false => NONEV end)  }>>.
 
   
-  Parameter markNode_proph_spec : ∀ Σ (H' : heapGS Σ) (n: Node) (p: proph_id) pvs,
+  Parameter markNode_proph_spec : ∀ Σ Hg1 (n: Node) (p: proph_id) pvs,
   ⊢ proph p pvs -∗ 
-    <<{ ∀∀ h mark next k, node Σ n h mark next k ∗ ⌜0 < h⌝ }>>
-          markNode #n #p @ ∅
+    <<{ ∀∀ h mark next k, node Σ Hg1 n h mark next k ∗ ⌜0 < h⌝ }>>
+          markNode' #n #p @ ∅
     <<{ ∃∃ (success: bool) mark' prf pvs',
-            node Σ n h mark' next k
+            node Σ Hg1 n h mark' next k
           ∗ proph p pvs'
           ∗ ⌜Forall (λ x, ∃ v1, x = ((v1, #false)%V, #())) prf⌝
           ∗ (match success with 
@@ -130,9 +124,9 @@ Module Type NODE_IMPL.
             RET (match success with true => SOMEV #() 
                                   | false => NONEV end)  }>>.
 
-  Parameter getHeight_spec : ∀ Σ (H' : heapGS Σ) (n: Node) (i: nat),
-    ⊢ <<{ ∀∀ h mark next k, node Σ n h mark next k }>>
+  Parameter getHeight_spec : ∀ Σ Hg1 (n: Node),
+    ⊢ <<{ ∀∀ h mark next k, node Σ Hg1 n h mark next k }>>
           getHeight #n @ ∅
-      <<{ node Σ n h mark next k | RET #h }>>.
+      <<{ node Σ Hg1 n h mark next k | RET #h }>>.
 
 End NODE_IMPL.
